TransVal/freeVars.v
@@ -1,0 +1,20 @@
+Require Import List smt Exp Util CSet.
+
+Fixpoint freeVars (s:smt) :=
+match s with
+| smtReturn e => Exp.freeVars e
+| funcApp f x => list_union (List.map (Exp.freeVars) x)
+| smtAnd a b => freeVars a ∪ freeVars b
+| smtOr a b => freeVars a ∪ freeVars b
+| smtNeg a => freeVars a
+| ite c t f => freeVars t ∪ freeVars f ∪ Exp.freeVars c
+| smtImp a b => freeVars a ∪ freeVars b
+| smtFalse => {}
+|constr e1 e2 => Exp.freeVars e1 ∪ Exp.freeVars e2
+end.
+
+(*
+*** Local Variables: ***
+*** coq-load-path: (("../" "Lvc")) ***
+*** End: ***
+*)
